lib/Crypto.s.dfy
@@ -1,0 +1,8 @@
+include "NativeTypes.s.dfy"
+
+module Crypto {
+  import opened NativeTypes
+
+  function method {:axiom} Sha256(t: seq<byte>) : (hash : seq<byte>)
+  ensures |hash| == 32
+}
